Rework GVT proofs with Fernand

case_study/RiscvPmp/BlockVer/PartialVerifier.v
@@ -316,25 +316,25 @@ Section BlockVerificationDerived.
 
     Context {Σ} {GS : sailGS Σ} {rG : iostateG IOState Σ}.
 
-    Fixpoint ptsto_instrs (a : Val ty_word) (instrs : list AST) : iProp Σ :=
+    Fixpoint ptsto_instrs (a : Val ty_xlenbits) (instrs : list AST) : iProp Σ :=
       match instrs with
       | cons inst insts => (interp_ptsto_instr a inst ∗ ptsto_instrs (bv.add a bv_instrsize) insts)%I
       | nil => True%I
       end.
     (* Arguments ptsto_instrs {Σ H} a%_Z_scope instrs%_list_scope : simpl never. *)
 
-    Definition blockVerifierAssumptions `{sailGS Σ} (PRE : (Val ty_xlenbits) → iProp Σ) (a : Val ty_xlenbits) : iProp Σ :=
-    (PRE a) ∗ pc ↦ᵣ a ∗ (∃ v, nextpc ↦ᵣ v).
+    Definition blockVerifierAssumptions `{sailGS Σ} (a : Val ty_xlenbits) : iProp Σ :=
+      pc ↦ᵣ a ∗ (∃ v, nextpc ↦ᵣ v).
 
     Definition semTripleOneInstrStep (PRE : iProp Σ) (instr : AST) (POST : Val ty_word -> iProp Σ) (a : Val ty_word) : iProp Σ :=
-      semTriple [env] (PRE ∗ (∃ v, lptsreg nextpc v) ∗ lptsreg pc a ∗ interp_ptsto_instr a instr)
+      semTriple [env] (PRE ∗ blockVerifierAssumptions a ∗ interp_ptsto_instr a instr)
         (FunDef RiscvPmpProgram.step)
         (fun ret _ => (∃ an, lptsreg nextpc an ∗ lptsreg pc an ∗ POST an) ∗ interp_ptsto_instr a instr)%I.
 
     Definition semTripleBlock (PRE : Val ty_word -> iProp Σ) (instrs : list AST) (POST : Val ty_word -> Val ty_word -> iProp Σ) : iProp Σ :=
       (∀ a,
-         (PRE a ∗ pc ↦ᵣ a ∗ (∃ v, nextpc ↦ᵣ v) ∗ ptsto_instrs a instrs) -∗
-         (∀ an, pc ↦ᵣ an ∗ (∃ v, nextpc ↦ᵣ v) ∗ ptsto_instrs a instrs ∗ POST a an -∗ WP_loop) -∗
+         (PRE a ∗ blockVerifierAssumptions a ∗ ptsto_instrs a instrs) -∗
+         (∀ an, blockVerifierAssumptions an ∗ ptsto_instrs a instrs ∗ POST a an -∗ WP_loop) -∗
          WP_loop)%I.
     #[global] Arguments semTripleBlock PRE%_I instrs POST%_I.
 
@@ -355,7 +355,7 @@ Section BlockVerificationDerived.
              produce_chunk lift_purespec CPureSpec.produce_chunk CPureSpec.pure
              CPureSpec.demonic CStoreSpec.evalStoreSpec].
       cbn - [consume].
-      iIntros (Hverif) "(Hheap & [%npc Hnpc] & Hpc & Hinstrs)".
+      iIntros (Hverif) "(Hheap & (Hpc & [%npc Hnpc]) & Hinstrs)".
       specialize (Hverif npc). apply sound_cexec in Hverif.
       iApply (semWP_mono with "[-]").
       iApply (sound_stm foreignSemBlockVerif lemSemBlockVerif Hverif with "[] [$]").
@@ -369,19 +369,19 @@ Section BlockVerificationDerived.
 
     Lemma sound_exec_block_addr {instrs ainstr apc} Φ (h : SCHeap) :
       cexec_block_addr instrs ainstr apc Φ h ->
-      interpret_scheap h ∗ lptsreg pc apc ∗ (∃ v, lptsreg nextpc v) ∗ ptsto_instrs ainstr instrs ⊢
-      (∀ an, lptsreg pc an ∗ (∃ v, lptsreg nextpc v) ∗ ptsto_instrs ainstr instrs ∗
+      interpret_scheap h ∗ blockVerifierAssumptions apc ∗ ptsto_instrs ainstr instrs ⊢
+      (∀ an, blockVerifierAssumptions an ∗ ptsto_instrs ainstr instrs ∗
              (∃ h', interpret_scheap h' ∧ ⌜Φ an h'⌝) -∗ WP_loop) -∗ WP_loop.
     Proof.
       revert ainstr apc Φ h.
       induction instrs as [|instr instrs]; cbn; intros ainstr apc Φ h;
         cbv [bind assert_formula lift_purespec CPureSpec.assert_formula
                CPureSpec.assert_pathcondition pure CPureSpec.pure].
-      - intros HΦ. iIntros "(Hpre & Hpc & Hnpc & _) Hk".
+      - intros HΦ. iIntros "(Hpre & (Hpc & Hnpc) & _) Hk".
         iApply "Hk"; iFrame; auto.
       - intros [-> Hverif%sound_exec_instruction].
         unfold semTripleOneInstrStep, semTriple in Hverif.
-        iIntros "(Hh & Hpc & Hnpc & Hinstr & Hinstrs) Hk".
+        iIntros "(Hh & (Hpc & Hnpc) & Hinstr & Hinstrs) Hk".
         iApply semWP_seq.
         iApply semWP_call_inline.
         iApply (semWP_mono with "[-Hinstrs Hk] [Hinstrs Hk]").
@@ -394,7 +394,7 @@ Section BlockVerificationDerived.
         iApply (semWP_call_inline loop).
         iApply (IHinstrs with "[$Hh' $Hpc Hnpc $Hinstrs]").
         { now iExists an. }
-        iIntros (an2) "(Hpc & Hnpc & Hinstrs & HPOST)".
+        iIntros (an2) "((Hpc & Hnpc) & Hinstrs & HPOST)".
         iApply ("Hk" with "[$]").
     Qed.
 
@@ -404,13 +404,13 @@ Section BlockVerificationDerived.
           (λ a na : Val ty_word, asn.interpret post (ι.[("a"::ty_xlenbits) ↦ a].[("an"::ty_xlenbits) ↦ na])).
     Proof.
       cbv [cexec_triple_addr bind demonic_ctx demonic CPureSpec.demonic lift_purespec].
-      iIntros (Htrip a) "(Hpre & Hpc & Hnpc & Hinstrs) Hk".
+      iIntros (Htrip a) "(Hpre & (Hpc & Hnpc) & Hinstrs) Hk".
       rewrite CPureSpec.wp_demonic_ctx in Htrip.
       specialize (Htrip ι a). apply produce_sound in Htrip.
       iPoseProof (Htrip with "[$] Hpre") as "(%h2 & [Hh2 %Hexec])". clear Htrip.
       apply sound_exec_block_addr in Hexec.
       iApply (Hexec with "[$]"). clear Hexec.
-      iIntros (an2) "(Hpc & Hnpc & Hinstrs & (%h3 & [Hh3 %Hconsume]))".
+      iIntros (an2) "((Hpc & Hnpc) & Hinstrs & (%h3 & [Hh3 %Hconsume]))".
       apply consume_sound in Hconsume.
       iPoseProof (Hconsume with "Hh3") as "[HPOST Hheap]".
       iApply ("Hk" with "[$]").
@@ -696,55 +696,57 @@ Section AnnotatedBlockVerification.
       | AnnotAST a => Some a
       | _ => None
       end.
+    Definition filter_AnnotInstr_AST (l : list AnnotInstr) :=
+      base.omap extract_AST l.
 
     Lemma sound_exec_annotated_block_addr {instrs ainstr apc} (h : SCHeap) (POST : Val ty_xlenbits -> iProp Σ) :
       LemmaSem ->
       cexec_annotated_block_addr instrs ainstr apc (fun res h' => interpret_scheap h' ⊢ POST res) h ->
-      ⊢ ((interpret_scheap h ∗ lptsreg pc apc ∗ (∃ v, lptsreg nextpc v) ∗ ptsto_instrs ainstr (omap extract_AST instrs)) -∗
-         (∀ an, lptsreg pc an ∗ (∃ v, lptsreg nextpc v) ∗ ptsto_instrs ainstr (omap extract_AST instrs) ∗ POST an -∗ WP_loop) -∗
+      ⊢ ((interpret_scheap h ∗ blockVerifierAssumptions apc ∗ ptsto_instrs ainstr (filter_AnnotInstr_AST instrs)) -∗
+         (∀ an, blockVerifierAssumptions an ∗ ptsto_instrs ainstr (filter_AnnotInstr_AST instrs) ∗ POST an -∗ WP_loop) -∗
          WP_loop)%I.
     Proof.
       intros lemSem.
       revert ainstr apc h POST.
       induction instrs as [|instr instrs]; cbn; intros ainstr apc h POST.
-      - iIntros (->) "(Hpre & Hpc & Hnpc & _) Hk".
+      - iIntros (->) "(Hpre & (Hpc & Hnpc) & _) Hk".
         iApply "Hk"; iFrame.
       - cbv [bind assert_formula lift_purespec CPureSpec.assert_formula
                CPureSpec.assert_pathcondition].
         destruct instr as [instr| |Δ lem es].
         + intros [-> Hverif]. cbn [extract_AST ptsto_instrs].
-          iIntros "(Hh & Hpc & Hnpc & Hinstr & Hinstrs) Hk".
+          iIntros "(Hh & (Hpc & Hnpc) & Hinstr & Hinstrs) Hk".
           iApply semWP_seq.
           iApply semWP_call_inline.
           iApply (semWP_mono with "[-Hinstrs Hk]").
           { iApply (sound_exec_instruction Hverif). iFrame. }
           clear Hverif.
-          iIntros ([v|m] _); last (iIntros "_"; now rewrite semWP_fail);
-            iIntros "([%an (Hnpc & Hpc & (%h2 & Hh2 & %Hverif))] & Hinstr)".
+          iIntros ([v|m] _); last (iIntros "_"; now rewrite semWP_fail).
+          iIntros "([%an (Hnpc & Hpc & (%h2 & Hh2 & %Hverif))] & Hinstr)".
           iApply (semWP_call_inline loop).
           specialize (IHinstrs _ _ _ _ Hverif).
           iApply (IHinstrs with "[$Hh2 $Hpc Hnpc $Hinstrs]").
           by iExists _.
-          iIntros (an2) "(Hpc & Hnpc & Hinstrs & HPOST)".
+          iIntros (an2) "(Hblockver & Hinstrs & HPOST)".
           iApply ("Hk" with "[$]").
         + cbv [debug pure lift_purespec CPureSpec.pure].
-          iIntros (->) "(Hh & Hpc & Hnpc & Hinstrs) Hk".
-          now iApply ("Hk" with "[$Hpc $Hnpc $Hinstrs Hh]").
-        + iIntros (Hlemcall) "(Hh & Hpc & Hnpc & Hinstrs) Hk".
+          iIntros (->) "(Hh & Hblockver & Hinstrs) Hk".
+          now iApply ("Hk" with "[$Hblockver $Hinstrs Hh]").
+        + iIntros (Hlemcall) "(Hh & Hblockver & Hinstrs) Hk".
           pose proof (Hlem := lemSem _ lem).
           apply call_lemma_sound in Hlemcall. destruct Hlemcall. cbn in *.
           iPoseProof (H with "Hh") as "(%ι & %Heq & Hreq & Hk2)". clear H.
           iPoseProof (Hlem with "Hreq") as "Hens".
           iPoseProof ("Hk2" with "Hens") as "(%h' & Hh' & %Hk2)".
           apply IHinstrs in Hk2.
-          iApply (Hk2 with "[$Hh' $Hpc $Hnpc $Hinstrs] Hk").
+          iApply (Hk2 with "[$Hh' $Hblockver $Hinstrs] Hk").
     Qed.
 
     Definition semTripleAnnotatedBlock (PRE : Val ty_word -> iProp Σ)
       (instrs : list AnnotInstr) (POST : Val ty_word -> Val ty_word -> iProp Σ) : iProp Σ :=
       (∀ a,
-         (PRE a ∗ pc ↦ᵣ a ∗ (∃ v, nextpc ↦ᵣ v) ∗ ptsto_instrs a (omap extract_AST instrs)) -∗
-         (∀ an, pc ↦ᵣ an ∗ (∃ v, nextpc ↦ᵣ v) ∗ ptsto_instrs a (omap extract_AST instrs) ∗ POST a an -∗ WP_loop) -∗
+         (PRE a ∗ blockVerifierAssumptions a ∗ ptsto_instrs a (filter_AnnotInstr_AST instrs)) -∗
+         (∀ an, blockVerifierAssumptions an ∗ ptsto_instrs a (filter_AnnotInstr_AST instrs) ∗ POST a an -∗ WP_loop) -∗
          WP_loop)%I.
     Global Arguments semTripleAnnotatedBlock PRE%_I instrs POST%_I.
 
@@ -756,14 +758,14 @@ Section AnnotatedBlockVerification.
           (λ a na : Val ty_word, asn.interpret post (ι.[("a"::ty_xlenbits) ↦ a].[("an"::ty_xlenbits) ↦ na])).
     Proof.
       intros lemSem Hexec ι.
-      iIntros (a) "(Hpre & Hpc & Hnpc & Hinstrs) Hk".
+      iIntros (a) "(Hpre & Hblockver & Hinstrs) Hk".
       hnf in Hexec.
       rewrite CPureSpec.wp_demonic_ctx in Hexec.
       specialize (Hexec ι a).
       unfold bind in Hexec.
       iPoseProof (produce_sound _ _ Hexec with "[//] [$Hpre]") as "(%h2 & Hh2 & %Hexec')".
       clear Hexec.
-      iApply (sound_exec_annotated_block_addr (apc := a) h2 with "[$Hh2 $Hpc $Hnpc $Hinstrs]"); auto.
+      iApply (sound_exec_annotated_block_addr (apc := a) h2 with "[$Hh2 $Hblockver $Hinstrs]"); auto.
       revert Hexec'.
       apply mono_cexec_annotated_block_addr.
       intros [? ?] ? <- h3 Hcons.
